src/examples.v
@@ -1,0 +1,260 @@
+Require Export Hoare.
+
+(*******************
+ * EXAMPLE 1       *
+ *******************)
+
+Definition body : com := 
+  Y ::= APlus (AId X) (ANum 1).
+
+Definition env : program :=
+  fun id =>
+    if eq_id_dec F id
+    then (body, [X], (APlus (AId X) (ANum 1)))
+    else (CSkip, [], ANum 0)
+    .
+
+Lemma body_p : forall X Y,
+  {{ (fun e st => st Y = st X + 1)[Y |-> (APlus (AId X) (ANum 1))] }}
+    Y ::= APlus (AId X) (ANum 1)
+  {{ (fun e st => st Y = st X + 1) }} env.
+Proof.
+  intros X Y.
+  apply hoare_consequence_post with (Q' := fun e st => st Y = st X + 1 /\ e = None).
+  eapply hoare_asgn.
+  intro; intros.
+  destruct H; assumption.
+Qed.
+
+(* Theorem prog_correct :
+  {{fun e st => True}}
+    CCall F Z [ANum 2]
+  {{fun e st => st Z = 3}} env.
+Proof.
+  eapply hoare_consequence_pre.
+  apply hoare_call with (params := [X]) (Q := fun e st => st Y = st X + 1)
+                  (body := body) (rexp := (APlus (AId X) (ANum 1)))
+                  (P := fun e st => st X = 2).
+  unfold env. simpl. reflexivity.
+  eapply hoare_consequence_pre.
+  apply hoare_consequence_post with (Q' := fun e st => st Y = st X + 1).
+  eapply body_p.
+  intro; intros.
+  simpl.
+  apply hoare_consequence_post
+  	with (Q' := fun e st => st Y = 3 /\ 3 = aeval st (APlus (AId X) (ANum 1)) /\ e = None).
+  apply hoare_asgn.
+  intro. intros _.
+  unfold assn_sub.
+  simpl.
+  split; try rewrite update_retrieve; reflexivity.
+Qed.
+
+( *******************
+ * EXAMPLE 2       *
+ ******************* )
+
+Definition Fbody : com := 
+  IFB (BEq (ANum 0) (AId X))
+  THEN Z ::= APlus (AId Y) (ANum 1)
+  ELSE CCall G Z [AId Y]
+  FI.
+  
+Definition Gbody : com := 
+  Z ::= APlus (AId Y) (ANum 1) ;;
+  Z ::= APlus (AId Z) (ANum 1)
+  .
+  
+Definition env'' : program :=
+  fun id =>
+    if eq_id_dec F id
+    then (Fbody, cons X (cons Y nil), (APlus (AId X) (AId Y)))
+    else if eq_id_dec G id
+    then (Gbody, [X], (APlus (AId X) (ANum 2)))
+    else (CSkip, [], ANum 0)  
+  .
+  
+Theorem prog_correct'' :
+  {{fun st => True}}
+    CCall F Z (cons (ANum 10) (cons (ANum 10) nil))
+  {{fun st => st Z = 20}} env''.
+Proof.
+  eapply hoare_consequence_pre.
+  apply hoare_call with (params := cons X (cons Y nil))
+			      (Q := fun st => st Z = st X + st Y)
+                  (body := Fbody) (rexp := (APlus (AId X) (AId Y)))
+                  (P := fun st => st X + st Y = st X + st Y /\ st X = 10 /\ st Y = 10).
+  unfold env''. simpl. reflexivity.
+  eapply hoare_consequence_post with (Q' := fun st => st Z = st X + st Y /\ st X = 10 /\ st Y = 10).
+  eapply hoare_consequence_pre with (P' := fun st => True).
+  unfold body''.
+  apply b''.
+  intro; intros; apply I.
+  intro; intros.
+  destruct H.
+  split. assumption.
+  unfold aeval. destruct H0; rewrite H0, H1; reflexivity.
+  intros st _. simpl.
+  split. reflexivity.
+  rewrite update_retrieve_dif, update_retrieve, update_retrieve.
+  split; reflexivity.
+  unfold Y, X, not; intro; congruence.
+Qed. *)
+
+Definition body'' : com := 
+  IFB (BEq (ANum 1) (AId X))
+  THEN Z ::= APlus (AId Y) (AId X)
+  ELSE CCall F Z (cons (AMinus (AId X) (ANum 1))
+				   (cons (APlus (AId Y) (ANum 1))
+ 					 nil))
+  FI.
+(*  
+Definition env'' : program :=
+  fun id =>
+    if eq_id_dec F id
+    then (body'', cons X (cons Y nil), (APlus (AId X) (AId Y)))
+    else (CSkip, [], ANum 0)
+    .
+
+( * 
+  {{ fun st => st X > 0 }} env
+  IFB (BEq (ANum 1) (AId X)) THEN
+    {{ fun st => st X = 1 /\ st X + Y = st X + Y }} env ->>
+    {{ fun st => st X + Y = st X + Y }} env
+    Z ::= APlus (AId X) (AId Y)
+    {{ fun st => st Z = st X + Y }} env
+  ELSE
+    {{ fun st => st X > 1 /\ st X + st Y = st X + st Y }} env
+    CCall F Z (cons (AMinus (AId X) (ANum 1))
+		   		 (cons (APlus (AId Y) (ANum 1))
+ 					nil))
+ 	{{ fun st => st X > 1 /\ st Z = st X + st Y }} env ->>
+ 	{{ fun st => st Z = st X + st Y }} env
+  FI.
+  {{ fun st => st Z = st X + st Y }} env * )
+
+Lemma b'' : forall X Y Z x y z env,
+  z = x + y ->
+  {{ (fun st => z = st Z /\ x = st X /\ y = st Y)[Z |-> APlus (AId Y) (AId X)] }}
+  IFB (BEq (ANum 1) (AId X))
+  THEN Z ::= APlus (AId Y) (AId X)
+  ELSE CCall F Z (cons (AMinus (AId X) (ANum 1))
+				   (cons (APlus (AId Y) (ANum 1))
+ 					 nil))
+  FI
+  {{ fun st => st Z = st X + st Y }} env.
+Proof.
+  intros X Y Z x y z env H.
+  apply hoare_if.
+  eapply hoare_consequence_post
+	with (Q' := fun st : state => st Z = st X + st Y).
+  eapply hoare_consequence_pre.
+  eapply hoare_asgn.
+  intro. intros.
+  unfold assn_sub in *.
+  destruct H0; destruct H0; destruct H2.
+  rewrite <- H0; rewrite <- H2; rewrite <- H3.
+  assumption.
+  intro; intros.
+  assumption.
+Admitted.
+
+Theorem prog_correct'' :
+  {{fun st => True}}
+    CCall F Z (cons (ANum 10) (cons (ANum 10) nil))
+  {{fun st => st Z = 20}} env''.
+Proof.
+  eapply hoare_consequence_pre.
+  apply call with (params := cons X (cons Y nil))
+			      (Q := fun st => st Z = st X + st Y)
+                  (body := body'') (rexp := (APlus (AId X) (AId Y)))
+                  (P := fun st => st X + st Y = st X + st Y /\ st X = 10 /\ st Y = 10).
+  unfold env''. simpl. reflexivity.
+  eapply hoare_consequence_post with (Q' := fun st => st Z = st X + st Y /\ st X = 10 /\ st Y = 10).
+  eapply hoare_consequence_pre with (P' := fun st => True).
+  unfold body''.
+  apply b''.
+  intro; intros; apply I.
+  intro; intros.
+  destruct H.
+  split. assumption.
+  unfold aeval. destruct H0; rewrite H0, H1; reflexivity.
+  intros st _. simpl.
+  split. reflexivity.
+  rewrite update_retrieve_dif, update_retrieve, update_retrieve.
+  split; reflexivity.
+  unfold Y, X, not; intro; congruence.
+Qed. *)
+
+( *******************
+ * EXAMPLE 3       *
+ ******************* )
+
+Definition example1 : com :=
+  X ::= ANum 3;;
+  TRY
+    X ::= ANum 4;;
+    THROW T, [AMinus (ANum 21) (AId X)];; (* Demonstrating the hoare_seq rule. *)
+    THROW U, [] (* Demonstrating the hoare_seq_exn rule. *)
+  CATCH T, [Y] DO (* Demonstrating the hoare_try_exn rule. *)
+    X ::= APlus (AId X) (AId Y)
+  END. (* {X = 20 /\ Y = 17} *)
+
+Definition example2 : com :=
+  X ::= ANum 2;;
+  TRY
+    X ::= ANum 18
+  CATCH T, [Y] DO (* Demonstrating the hoare_try rule. *)
+    X ::= AId Y
+  END. (* {X = 18} *)
+
+Definition example3 : com :=
+  X ::= ANum 2;;
+  TRY
+    X ::= ANum 18;;
+    THROW T, [ANum 4; ANum 3]
+  CATCH U, [Y; Z] DO (* Demonstrating the hoare_try rule with propagated exception. *)
+    X ::= APlus (AId Y) (AId Z)
+  END. (* {X = 2 /\ ex = Some (Exn (T, [4; 3]))} *)
+
+Theorem example1_correct :
+  {{fun ex st => True}}
+    example1
+  {{fun ex st => st X = 20 /\ st Y = 17}}.
+Proof.
+  unfold example1.
+  eapply hoare_consequence_pre.
+  apply hoare_seq with (Q:=fun ex st => st X = 3).
+  apply hoare_try_exn with (ns:=[17]).
+  apply hoare_consequence_post with (fun ex st => (st X = 20 /\ st Y = 17) /\ ex = None).
+  eapply hoare_consequence_pre. apply hoare_asgn.
+  intros ex st P.
+  unfold assn_sub. unfold aeval. unfold update.
+  inversion P. inversion H. clear H. split.
+  destruct (eq_id_dec X X).
+    rewrite H1. unfold update_many. simpl. unfold update.
+    destruct (eq_id_dec Y X). destruct (eq_id_dec Y Y).
+    inversion e0. congruence.
+    destruct (eq_id_dec Y Y). rewrite H0. reflexivity.
+    congruence. congruence.
+  destruct (eq_id_dec X Y).
+    rewrite H1. unfold update_many. simpl. unfold update.
+    destruct (eq_id_dec Y X). destruct (eq_id_dec Y Y).
+    inversion e0. congruence.
+    destruct (eq_id_dec Y Y); congruence.
+    rewrite H1. unfold update_many. simpl. unfold update.
+    destruct (eq_id_dec Y Y). reflexivity. congruence.
+  intros ex st P. omega.
+  apply hoare_seq with (fun ex st => st X = 4).
+  apply hoare_seq_exn.
+  eapply hoare_consequence_post. apply hoare_throw.
+  intros ex st P.
+  inversion P. clear P.
+  unfold map in H0. unfold aeval in H0. rewrite H in H0.
+  split. assumption. congruence.
+  eapply hoare_consequence_pre. apply hoare_asgn.
+  intros ex st P.
+  unfold assn_sub. unfold aeval. reflexivity.
+  apply hoare_asgn.
+  intros ex st P. unfold assn_sub. reflexivity.
+Qed.
